arith/ArithS.lean
@@ -69,6 +69,8 @@ import ArithS.Necessitation.Top
 import ArithS.Necessitation.PrologueRows
 import ArithS.Necessitation.Prologue
 import ArithS.Necessitation.NumId
+import ArithS.Necessitation.NumIdRows
+import ArithS.Necessitation.Pin
 import ArithS.Neg
 import ArithS.Agent
 import ArithS.AgentConverse
